Working out details

clrs/rbt_insert_gen.rkt
@@ -4,6 +4,7 @@
 (Fixpoint
  rbt_insert #:implicit @A{Set}
  @A_cmp{A -> A -> Prop}
+ @A_refl{forall x, A_cmp x x}
  @A_asym{forall x y, A_cmp x y -> ~ A_cmp y x}
  @A_trans{Transitive A A_cmp}
  @A_cmp_dec{forall (x y:A),
@@ -12,7 +13,7 @@
  @ct{CTree A} @x{A}
  #:returns @{CTree A}
  (bind 
-  ((ctp (rbt_insert_inner A_cmp A_asym A_trans A_cmp_dec A_eq_dec ct x)))
+  ((ctp (rbt_insert_inner A_cmp A_refl A_asym A_trans A_cmp_dec A_eq_dec ct x)))
   (bind 
    ((res (rbt_blacken ct)))
    (<== res))))
