clrs/rbt_insert_inner_gen.rkt
@@ -3,8 +3,10 @@
 (require "rbt_balance_gen.rkt")
 
 (Fixpoint
- rbt_insert_inner #:implicit @A{Set}
+ rbt_insert_inner
+ @A{Set}
  @A_cmp{A -> A -> Prop}
+ @A_refl{forall x, A_cmp x x}
  @A_asym{forall x y, A_cmp x y -> ~ A_cmp y x}
  @A_trans{Transitive A A_cmp}
  @A_cmp_dec{forall (x y:A),
@@ -15,7 +17,7 @@
  (match (ct)
    [(CT_leaf)
     =>
-    (<== (CT_node ct RED x ct))]
+    (<== (CT_node A ct RED x ct))]
    [(CT_node l c v r)
     =>
     (match ((A_eq_dec x v))
@@ -28,14 +30,14 @@
          [(left _)
           =>
           (bind 
-           ((lp (rbt_insert_inner A_cmp A_asym A_trans A_cmp_dec A_eq_dec l x)))
+           ((lp (rbt_insert_inner A A_cmp A_refl A_asym A_trans A_cmp_dec A_eq_dec l x)))
            (bind 
-            ((res (rbt_balance lp c x r)))
+            ((res (rbt_balance A lp c v r)))
             (<== res)))]
          [(right _)
           =>
           (bind 
-           ((rp (rbt_insert_inner A_cmp A_asym A_trans A_cmp_dec A_eq_dec r x)))
+           ((rp (rbt_insert_inner A A_cmp A_refl A_asym A_trans A_cmp_dec A_eq_dec r x)))
            (bind 
-            ((res (rbt_balance l c x rp)))
+            ((res (rbt_balance A l c v rp)))
             (<== res)))])])]))
